TestModels/dafny-dependencies/StandardLibrary/src/Actions/Aggregators.dfy
@@ -1,0 +1,109 @@
+include "Actions.dfy"
+include "../DynamicArray.dfy"
+
+module {:options "--function-syntax:4"} Std.Aggregators {
+
+  import opened Actions
+  import opened Wrappers
+  import opened DynamicArray
+
+  // TODO: Names need improvement
+  type IAggregator<T> = Action<T, ()>
+  type Aggregator<T> = Action<T, bool> // | exists limit: nat :: ProducesTerminatedBy(a, r => !r, limit) witness *
+  type Accumulator<T> = Action<Option<T>, ()> // | exists limit :: ConsumesTerminatedBy(a, None, limit) witness *
+  
+  class ArrayAggregator<T> extends Action<T, ()>, ConsumesAllProof<T, ()> {
+
+    var storage: DynamicArray<T>
+
+    ghost predicate Valid() 
+      reads this, Repr 
+      ensures Valid() ==> this in Repr 
+      ensures Valid() ==> 
+        && CanProduce(history)
+      decreases height, 0
+    {
+      && this in Repr
+      && storage in Repr
+      && this !in storage.Repr
+      && storage.Repr <= Repr
+      && storage.Valid?()
+      && Consumed() == storage.items
+    }
+
+    constructor() 
+      ensures Valid()
+      ensures fresh(Repr - {this})
+      ensures history == []
+    {
+      var a := new DynamicArray();
+
+      history := [];
+      height := 1;
+      Repr := {this} + {a} + a.Repr;
+      this.storage := a;
+    }
+
+    ghost predicate CanConsume(history: seq<(T, ())>, next: T)
+      decreases height
+    {
+      true
+    }
+    ghost predicate CanProduce(history: seq<(T, ())>)
+      decreases height
+    {
+      true
+    }
+
+    method Invoke(t: T) returns (r: ()) 
+      requires Requires(t)
+      modifies Modifies(t)
+      decreases Decreases(t).Ordinal()
+      ensures Ensures(t, r)
+    {
+      assert Consumed() == storage.items;
+      storage.Push(t);
+
+      r := ();
+      Update(t, r);
+      Repr := {this} + {storage} + storage.Repr;
+      assert Consumed() == old(Consumed()) + [t];
+      assert Valid();
+    }
+
+    method RepeatUntil(t: T, stop: (()) -> bool, ghost eventuallyStopsProof: ProducesTerminatedProof<T, ()>)
+      requires Valid()
+      requires eventuallyStopsProof.Action() == this
+      requires eventuallyStopsProof.FixedInput() == t
+      requires eventuallyStopsProof.StopFn() == stop
+      requires forall i <- Consumed() :: i == t
+      // reads Reads(t)
+      modifies Repr
+      ensures Valid()
+    {
+      DefaultRepeatUntil(this, t, stop, eventuallyStopsProof);
+    }
+
+    ghost function Action(): Action<T, ()> {
+      this
+    }
+
+    lemma CanConsumeAll(history: seq<(T, ())>, next: T) 
+      requires Action().CanProduce(history)
+      ensures Action().CanConsume(history, next) 
+    {
+    }
+  }
+
+  method {:rlimit 0} AggregatorExample() {
+    var a: ArrayAggregator<nat> := new ArrayAggregator();
+    var _ := a.Invoke(1);
+    var _ := a.Invoke(2);
+    var _ := a.Invoke(3);
+    var _ := a.Invoke(4);
+    var _ := a.Invoke(5);
+    var _ := a.Invoke(6);
+    assert a.Consumed() == [1, 2, 3, 4, 5, 6];
+    assert a.storage.items == [1, 2, 3, 4, 5, 6];
+  }
+}
